gc updates

src/Gc.v
@@ -6,6 +6,12 @@ Inductive addresing_string : Type :=
 | FollowStr : nat -> addresing_string -> addresing_string
 .
 
+Fixpoint address_length (address: addresing_string) : nat :=
+  match address with
+  | TermStr => 1
+  | FollowStr n rest => S (address_length rest)
+  end.
+
 Inductive addresses : heap_t -> ptr -> addresing_string -> ptr -> Prop :=
 | TermAddresses : forall h p,
     (exists vs, heap_maps_struct h p vs) ->
@@ -22,26 +28,640 @@ Fixpoint union_pointers (l : list (set ptr)) : set ptr :=
   | h::t => (set_union ptr_eq_dec h  (union_pointers t))
   end.
 
+Theorem nth_union_pointers:
+  forall l n p,
+    set_In p (nth n l (@nil ptr)) ->
+    set_In p (union_pointers l).
+Proof.
+  induction l ; induction n ; intros.
+  * inversion H.
+  * crush.
+  * crush.
+    eapply set_union_intro1. auto.
+  * crush.
+    specialize (IHl n p). intuition.
+    eapply set_union_intro2. auto.
+Qed.
+
+Theorem nth_union_pointers_inv:
+  forall l p,
+    set_In p (union_pointers l) ->
+    exists n, set_In p (nth n l (@nil nat)).
+Proof.
+  induction l. crush.
+  intros.
+  unfold union_pointers in H.
+  fold union_pointers in H.
+  specialize (set_union_elim ptr_eq_dec p a (union_pointers l) H).
+  intros.
+  destruct H0.
+  * exists 0.
+    crush.
+  * specialize (IHl p H0).
+    destruct IHl.
+    exists (S x).
+    crush.
+Qed.
+
+Lemma set_diff_union :
+  forall {A: Type} (eq_dec : forall (x y: A), {x = y} + {x <> y})
+         a b c,
+    length (set_diff eq_dec (set_union eq_dec a b) (set_union eq_dec a c)) =
+    length (set_diff eq_dec b c).
+Proof.
+Admitted.
+
+Lemma set_diff_union_rewrite :
+  forall {A: Type} (eq_dec : forall (x y: A), {x = y} + {x <> y})
+         a b c foo,
+  length (set_diff eq_dec (set_union eq_dec a b) (set_union eq_dec a c)) = foo ->
+  length (set_diff eq_dec b c) = foo.
+Proof.
+  intros.
+  specialize (set_diff_union eq_dec a b c).
+  crush.
+Qed.
+
+Lemma set_diff_union_rewrite_inv :
+  forall {A: Type} (eq_dec : forall (x y: A), {x = y} + {x <> y})
+         a b c foo,
+    length (set_diff eq_dec b c) = foo ->
+    length (set_diff eq_dec (set_union eq_dec a b) (set_union eq_dec a c)) = foo.
+Proof.
+  intros.
+  specialize (set_diff_union eq_dec a b c).
+  crush.
+Qed.
+
+  (*
+  induction a ; intros.
+  * admit.
+  * specialize IHa with b c.
+    unfold set_union in *. fold set_union in *.
+  * crush.
+  * crush.
+  * specialize IHb with nil.
+    assert ((set_union eq_dec nil nil) = nil). crush.
+    rewrite H in *. clear H.
+
+    assert ((length (set_diff eq_dec (a :: b) nil)) = length (a::b)).
+    unfold set_diff. destruct (set_mem eq_dec a nil) eqn:?. crush. crush.
+
+    unfold set_union. fold set_union.
+    unfold set_diff. fold set_diff.
+    destruct (set_mem eq_dec a nil) eqn:?. crush.
+    unfold set_add. fold set_add.
+  * admit.
+  * admit.
+  * admit.
+  * admit.
+  * admit.
+Qed.
+ *)
+
 Fixpoint mark_ptr (fuel:nat) (p: ptr) (h: heap_t) : set ptr :=
   match fuel, heap_get_struct p h with
   | S n, Some vs =>
       (set_union ptr_eq_dec (set_add ptr_eq_dec p (empty_set ptr))
-        (union_pointers 
+        (union_pointers
           (List.map
             (fun v =>
               match v with
-              | Int _ => List.nil
+              | Int _ => nil
               | Pointer p' => mark_ptr n p' h
               end
            ) vs)))
-  | _, _ => List.nil
+  | _, _ => nil
   end
 .
 
+Theorem mark_ptr_subset:
+  forall f e p h,
+    set_In e (mark_ptr f p h) ->
+    exists v, In (e, v) h.
+Proof.
+  induction f ; crush.
+  destruct (heap_get_struct p h) eqn:?.
+  specialize (set_union_elim _ _ _ _ H). intros.
+  destruct H0.
+  * exists l. unfold heap_get_struct.
+    clear IHf H.
+    induction h. crush. intros. destruct a.
+    unfold heap_get_struct in Heqo.
+    destruct (ptr_eq_dec p0 p) eqn:? ; crush.
+  * clear H.
+    specialize (nth_union_pointers_inv _ _ H0). intros. destruct H. clear H0.
+
+    specialize (@map_nth
+                  val
+                  (list ptr)
+                  (fun v : val =>
+                     match v with
+                     | Int _ => nil
+                     | Pointer p' => mark_ptr f p' h
+                     end) l (Int 0) x).
+  unfold ptr. unfold set.
+  unfold ptr in H. unfold set in H.
+  intros. rewrite H0 in H. clear H0.
+  destruct (nth x l (Int 0)). crush.
+  eapply IHf. apply H.
+  * crush.
+Qed.
+
+Theorem mark_ptr_monotonic_1 :
+  forall f e p h,
+  set_In e (mark_ptr f p h) ->
+  set_In e (mark_ptr (S f) p h).
+Proof.
+  induction f. crush.
+  intros.
+  specialize (IHf e).
+  unfold mark_ptr in H.
+  fold mark_ptr in H.
+  unfold mark_ptr.
+  fold mark_ptr.
+  destruct (heap_get_struct p h). Focus 2. crush.
+  specialize (set_union_elim _ _ _ _ H). intros. destruct H0.
+  inversion H0. eapply set_union_intro1. crush.
+  inversion H1.
+  eapply set_union_intro2.
+
+  specialize (nth_union_pointers_inv _ _ H0). intros. destruct H1. clear H0.
+  eapply (nth_union_pointers _ x).
+
+  specialize (@map_nth
+                val
+                (list ptr)
+                (fun v : val =>
+           match v with
+           | Int _ => nil
+           | Pointer p' =>
+               match heap_get_struct p' h with
+               | Some vs =>
+                   set_union ptr_eq_dec (set_add ptr_eq_dec p' (empty_set ptr))
+                     (union_pointers
+                        (map
+                           (fun v0 : val =>
+                            match v0 with
+                            | Int _ => nil
+                            | Pointer p'0 => mark_ptr f p'0 h
+                            end) vs))
+               | None => nil
+               end
+           end) l (Int 0) x).
+  unfold ptr. unfold set.
+  intros. rewrite H0. clear H0.
+
+  specialize (@map_nth
+                val
+                (list ptr)
+                (fun v : val =>
+                match v with
+                | Int _ => nil
+                | Pointer p' => mark_ptr f p' h
+                end) l (Int 0) x).
+  unfold ptr. unfold set.
+  unfold ptr in H1. unfold set in H1.
+  intros. rewrite H0 in H1. clear H0.
+  destruct (nth x l (Int 0)). crush.
+  specialize (IHf p0 h H1).
+  auto.
+Qed.
+
+Theorem mark_ptr_monotonic_2 :
+  forall f f' e p h,
+    set_In e (mark_ptr f p h) ->
+    f <= f' ->
+    set_In e (mark_ptr f' p h).
+Proof.
+  induction f'.
+  * intros.
+    inversion H0.
+    crush.
+  * intros.
+    specialize (IHf' e p h). intuition.
+    inversion H0.
+    - subst. auto.
+    - intuition.
+      eapply mark_ptr_monotonic_1.
+      auto.
+Qed.
+Theorem mark_ptr_saturates_1 :
+  forall f p h,
+    length (set_diff ptr_eq_dec (mark_ptr (S f) p h) (mark_ptr f p h)) = 0 ->
+    length (set_diff ptr_eq_dec (mark_ptr (S (S f)) p h) (mark_ptr (S f) p h)) = 0.
+Proof.
+  Admit.
+
+
+
+  induction f.
+  * admit.
+  * intros.
+    unfold mark_ptr in H ; fold mark_ptr in H.
+    unfold mark_ptr ; fold mark_ptr.
+    destruct (heap_get_struct p h). Focus 2. crush.
+    specialize (set_diff_union_rewrite _ _ _ _ _ H). clear H. intros.
+    eapply set_diff_union_rewrite_inv.
+    induction l.
+    - crush.
+    -
+      eapply IHf.
+
+
+
+    specialize (set_diff_union_rewrite _ _ _ _ _ H). clear H. intros.
+    specialize (set_diff_union ptr_eq_dec
+                               (set_add ptr_eq_dec p (empty_set ptr)) (union_pointers
+                 (map
+                    (fun v : val =>
+                     match v with
+                     | Int _ => nil
+                     | Pointer p' =>
+                         match heap_get_struct p' h with
+                         | Some vs =>
+                             set_union ptr_eq_dec
+                               (set_add ptr_eq_dec p' (empty_set ptr))
+                               (union_pointers
+                                  (map
+                                     (fun v0 : val =>
+                                      match v0 with
+                                      | Int _ => nil
+                                      | Pointer p'0 => mark_ptr f p'0 h
+                                      end) vs))
+                         | None => nil
+                         end
+                     end) l)) (union_pointers
+                 (map
+                    (fun v : val =>
+                     match v with
+                     | Int _ => nil
+                     | Pointer p' => mark_ptr f p' h
+                     end) l))).
+    unfold ptr in *.
+    unfold set in *.
+    intros.
+    rewrite H0 in H.
+    clear H0.
+    eapply set_diff_union.
+
+Admitted.
+
+Theorem mark_ptr_saturates_1 :
+  forall f p h,
+    length (mark_ptr (S f) p h) = length (mark_ptr f p h) ->
+    length (mark_ptr (S (S f)) p h) = length (mark_ptr f p h).
+Proof.
+  induction f.
+  * crush.
+    destruct (heap_get_struct p h).
+    - admit.
+    - auto.
+  * intros.
+
+Qed.
+
+
+Theorem mark_ptr_saturates_1 :
+  forall h e p,
+  exists f,
+    set_In e (mark_ptr (S f) p h) ->
+    set_In e (mark_ptr f p h).
+Proof.
+Admitted.
+
+(* each addition fuel gives it at least one, up until it saturates *)
+(* highest anything can saturate is length *)
+
+Theorem mark_ptr_saturates_1 :
+  forall h e p,
+    set_In e (mark_ptr (S (length h)) p h) ->
+    set_In e (mark_ptr (length h) p h).
+Proof.
+  intros.
+
+  destruct (set_In_dec ptr_eq_dec e (mark_ptr (length h) p h)). auto.
+  contradict n.
+  intros.
+  remember (length h) as n.
+  revert Heqn H.
+  induction n.
+  * crush. admit.
+  * intros.
+  unfold mark_ptr in H ; fold mark_ptr in H.
+  assert (exists n, (length h = S n)). destruct h. crush. exists (length h). crush.
+
+  destruct H0.
+
+  induction x.
+  * rewrite H0. unfold mark_ptr ; fold mark_ptr.
+    destruct (heap_get_struct p h) eqn:?. Focus 2. crush.
+    destruct (ptr_eq_dec p e) eqn:?.
+    - eapply set_union_intro1. crush.
+    - eapply set_union_intro2.
+      specialize (set_union_elim _ _ _ _ H). intros. destruct H1.
+      + inversion H1. Focus 2. crush. crush.
+      + clear H.
+
+        specialize (nth_union_pointers_inv _ _ H1). intros. destruct H. clear H1.
+        specialize (@map_nth
+                      val
+                      (list ptr)
+                      (fun v : val =>
+                         match v return list ptr with
+                         | Int _ => nil
+                         | Pointer p' => mark_ptr (length h) p' h
+                         end) l (Int 0) x).
+        unfold ptr. unfold set.
+        unfold ptr in H. unfold set in H.
+        intros.
+        rewrite H1 in H.
+        clear H1.
+        eapply (nth_union_pointers _ x).
+        specialize (@map_nth
+                      val
+                      (list ptr)
+                      (fun v : val =>
+                         match v return list ptr with
+                         | Int _ => nil
+                         | Pointer p' => nil
+                         end) l (Int 0) x).
+        unfold ptr. unfold set.
+        intros.
+        rewrite H1.
+        clear H1.
+        destruct (nth x l (Int 0)). crush.
+        unfold ptr in H. unfold ptr in H0.
+        rewrite H0 in H.
+        unfold mark_ptr in H.
+        admit.
+  *
+
+        specialize (
+
+        rewrite H0 in H1. unfold mark_ptr in H1 ; fold mark_ptr in H1.
+
+        subst.
+        eapply set_union_intro1. crush.
+    - eapply set_union_intro2. clear H.
+
+
+  rewrite H0. unfold mark_ptr ; fold mark_ptr.
+  destruct (heap_get_struct p h) eqn:?. Focus 2. crush.
+  specialize (set_union_elim _ _ _ _ H). intros. destruct H1.
+  * inversion H1. Focus 2. crush.
+    subst.
+    eapply set_union_intro1. crush.
+  * eapply set_union_intro2. clear H.
+
+
+ edestruct (heap_get_struct p h) eqn:?. unfold heap_get_
+
+  destruct (set_In_dec ptr_eq_dec e (mark_ptr (length h) p h)). auto.
+  specialize (mark_ptr_monotonic_3 (length h) e p h H n).
+  intros.
+  destruct H0. destruct H0. destruct H0.
+
+  induction h. crush.
+  intuition.
+
+
+  induction h.
+  * intros. crush.
+  * intros.
+    assert (length (a::h) = S (length h)). crush. rewrite H0. clear H0.
+    unfold mark_ptr ; fold mark_ptr.
+
+
+
+  pose (0:nat).
+  intros h.
+  assert (length h = length h - n). crush.
+  rewrite H.
+  induction n.
+  * intros.
+    rewrite H.
+
+  intros h.
+  pose ((length h):nat).
+  assert (n = length h). crush.
+  rewrite <- H.
+  assert (n >= length h). crush. clear H.
+  induction n. assert (length h = 0). inversion H0. crush. assert (h = nil). eapply length_zero_iff_nil. crush. crush.
+  intros.
+  destruct (PeanoNat.Nat.eq_dec n (length h)).
+  * subst.
+    assert (length h >= length h). crush.
+    intuition. clear H1.
+    specialize (H2 e p).
+  *
+
+  induction (length h) eqn:? ; intros. assert (h = nil). eapply length_zero_iff_nil. crush. crush.
+
+  crush.
+
+  destruct h. crush.
+  assert (length (p0::h) = S (length h)). crush. rewrite H1. clear H1.
+  destruct p0.
+
+  unfold mark_ptr in H ; fold mark_ptr in H.
+  unfold mark_ptr ; fold mark_ptr.
+  destruct (heap_get_struct p ((p0, l) :: h)).
+  * specialize (set_union_elim _ _ _ _ H). intros. destruct H1.
+    - eapply set_union_intro1. crush.
+    - eapply set_union_intro2.
+      clear H.
+      specialize (nth_union_pointers_inv _ _ H1). intros. destruct H. clear H1.
+      eapply (nth_union_pointers _ x).
+
+      specialize (@map_nth
+                    val
+                    (list ptr)
+                    (fun v : val =>
+                       match v return list ptr with
+                       | Int _ => nil
+                       | Pointer p' => mark_ptr (length h) p' ((p0,l)::h)
+                       end) l0 (Int 0) x).
+      intros. rewrite H1. clear H1.
+
+      specialize (@map_nth
+                    val
+                    (list ptr)
+                    (fun v : val =>
+                       match v return list ptr with
+                       | Int _ => nil
+                       | Pointer p' => mark_ptr f p' ((p0,l)::h)
+                       end) l0 (Int 0) x).
+      intros.
+      unfold ptr in H; unfold ptr in H1 ; unfold set in H ; unfold set in H1.
+      rewrite H1 in H. clear H1.
+      destruct (nth x l0 (Int 0)). crush.
+      specialize (IHf ((p0,l)::h) e p1). intuition.
+      destruct (Compare_dec.le_gt_dec f (length ((p0,l) :: h))).
+      + assert (f = length ((p0, l) :: h)). crush.
+        subst. clear H0 l1 H1.
+Admitted.
+(*
+        eapply mark_ptr_saturates_1.
+      + intuition.
+      eapply IHf.
+  * crush.
+Qed.
+  intros.
+  assert (exists n, length h = S n). destruct h. crush. exists (length h). crush.
+  destruct H1.
+  specialize (IHf h e).
+  rewrite H1 in *. clear H1.
+  clear IHf.
+  induction x ; induction f ; try solve [crush].
+  *
+  rewrite H1.
+  destruct (Compare_dec.gt_dec f (S x)). Focus 2. assert (f = S x). crush. subst. clear n. clear H0. rewrite <- H1 in *. clear H1. clear IHf.
+  admit.
+  specialize (IHf p).
+  eapply IHf.
+
+  * admit.
+  *
+  unfold mark_ptr in *. fold mark_ptr in *.
+  specialize (IHf h e p).
+
+  induction h. intros. assert (exists f', f = S f'). inversion H0. crush. crush. crush.
+  intros.
+  assert (length (a::h) = S (length h)). crush. rewrite H1. clear H1.
+
+  induction f. crush.
+  intros.
+
+
+  intros.
+  eapply IHf.
+
+  destruct h. crush.
+  intros.
+
+  assert (length (a::h) = S (length h)). crush. rewrite H1. clear H1.
+  unfold mark_ptr in * ; fold mark_ptr in *.
+
+  unfold mark_ptr.
+Qed.
+
+Theorem mark_ptr_saturates :
+  forall f h e p,
+    set_In e (mark_ptr f p h) ->
+    set_In e (mark_ptr (length h) p h).
+Proof.
+  induciton f
+
+
+  induction f ; induction h ; try solve [crush].
+  intros.
+  assert (length (a::h) = S (length h)). crush. rewrite H0. clear H0.
+  unfold mark_ptr in * ; fold mark_ptr in *.
+  destruct a.
+  destruct (ptr_eq_dec p0 p) eqn:?.
+  * unfold heap_get_struct in *. rewrite Heqs in *.
+    destruct (ptr_eq_dec e p) eqn:?.
+    - eapply set_union_intro1. crush.
+    - eapply set_union_intro2.
+      specialize (set_union_elim ptr_eq_dec _ _ _ H).
+      intros.
+      destruct H0 ; crush.
+      specialize (nth_union_pointers_inv _ _ H0).
+      intros. destruct H1.
+      eapply (nth_union_pointers _ x).
+      specialize (@map_nth
+                    val
+                    (list ptr)
+                    (fun v : val =>
+                       match v return list ptr with
+                       | Int _ => nil
+                       | Pointer p' => mark_ptr (length h) p' ((p,l)::h)
+                     end) l (Int 0) x).
+      intros. rewrite H2 ; clear H2.
+
+      specialize (@map_nth
+                    val
+                    (set ptr)
+                    (fun v : val =>
+                       match v with
+                       | Int _ => nil
+                       | Pointer p' => mark_ptr f p' ((p, l) :: h)
+                       end) l (Int 0) x).
+      intros. intuition.
+      unfold set in H1.
+      unfold set in H2.
+      unfold ptr in H2.
+      unfold ptr in H1.
+      rewrite H2 in H1. clear H2.
+      specialize (nth_default_eq x l (Int 0)). intros.
+      rewrite <- H2. rewrite <- H2 in H1. intros. clear H2.
+      destruct (nth_default (Int 0) l x) eqn:?. crush.
+
+      specialize (nth_default_eq x l (Int 0)). intros.
+      unfold n
+
+      specialize (@nth_default_eq (set ptr) x (map
+               (fun v : val =>
+                match v with
+                | Int _ => nil
+                | Pointer p' => mark_ptr f p' ((p, l) :: h)
+                end) l) (@nil nat)).
+      intros.
+      rewrite <- H2 in H1.
+      clear H2.
+
+      destruct ((@nth_default (set ptr) (@nil nat)
+            (@map val (list ptr)
+               (fun v : val =>
+                match v return (list ptr) with
+                | Int _ => @nil ptr
+                | Pointer p' =>
+                    mark_ptr f p'
+                      (@cons (prod ptr (list val)) (@pair ptr (list val) p l) h)
+                end) l) x)). crush
+      destruct ((nth_default nil
+            (map
+               (fun v : val =>
+                match v with
+                | Int _ => nil
+                | Pointer p' => mark_ptr f p' ((p, l) :: h)
+                end) l) x)) eqn:?.
+      rewrite Heql0 in H1.
+
+      edestruct nth_default eqn:?. crush.
+
+      specialize (@map_nth
+                    val
+                    (list ptr)
+                    (fun v : val =>
+                       match v return list ptr with
+                       | Int _ => @nil ptr
+                       | Pointer p' => mark_ptr f p' ((p,l)::h)
+                       end) l (Int 0) x).
+      intros. intuition.
+      rewrite H2 in H1.
+
+      specialize (map_ne
+      unfold nth_default. rewrite H0.
+      specailze
+      eapply IHh.
+Admitted.
+(*
+  induction f ; induction h ; crush.
+  destruct (ptr_eq_dec a0 p) eqn:?.
+  *
+  * crush.
+  * induction h.
+  - crush.
+  - intros.
+Admitted.
+*)
+*)
 Theorem mark_ptr_marks :
   forall address h p p',
     addresses h p address p' ->
-    exists f, set_In p' (mark_ptr f p h)
+    set_In p' (mark_ptr (List.length h) p h)
 .
 Proof.
   induction address.
@@ -49,32 +669,42 @@ Proof.
     inversion H. clear H.
     inversion H0. clear H0.
     subst.
-    exists 1.
-    unfold mark_ptr.
-    rewrite H.
-    apply set_union_iff; crush.
+    induction h.
+    - inversion H.
+    - assert (length (a :: h) = S (length h)) ; auto.
+      rewrite H0.
+      unfold mark_ptr.
+      rewrite H.
+      apply set_union_iff; crush.
   * intros.
-    inversion H. clear H.
+    inversion H.
     subst.
     specialize (IHaddress h p'0 p' H6).
-    inversion IHaddress. clear IHaddress.
-    exists (S x).
-    specialize (heap_maps_implies_heap_get h p n (Pointer p'0) H4).
-    intros.
-    inversion H0 ; clear H0.
-    destruct H1.
-    unfold mark_ptr.
-    fold mark_ptr.
-    rewrite H0.
-    specialize (List.map_nth_error (fun v : val =>
-           match v with
-           | Int _ => nil
-           | Pointer p'1 => mark_ptr x p'1 h
-           end) n x0 H1).
-    intros.
-    apply set_union_iff.
-    crush.
-Admitted.
+    assert (exists n0, set_In p' (mark_ptr n0 p h)).
+    - exists (S (length h)).
+      unfold mark_ptr ; fold mark_ptr.
+      specialize (heap_maps_implies_heap_get h p n (Pointer p'0) H4).
+      intros. destruct H0. destruct H0.
+      rewrite H0.
+      eapply set_union_intro2.
+      eapply (nth_union_pointers _ n).
+
+      specialize (@map_nth
+                    val
+                    (list ptr)
+                    (fun v : val =>
+                       match v return list ptr with
+                       | Int _ => nil
+                       | Pointer p'1 => mark_ptr (length h) p'1 h
+                     end) x (Int 0) n).
+      intros. rewrite H2 ; clear H2.
+      specialize (nth_default_eq n x (Int 0)). intros.
+      rewrite <- H2. intros. clear H2.
+      unfold nth_default. rewrite H1.
+      auto.
+    - destruct H0.
+      eapply mark_ptr_saturates. apply H0.
+Qed.
 
 Theorem mark_ptr_correct :
   forall h p p' f,
@@ -99,7 +729,7 @@ Proof.
     clear e.
     apply set_union_iff in H.
     destruct H.
-    * crush. 
+    * crush.
       eauto.
     * dependent induction l.
       + crush.
@@ -123,11 +753,11 @@ Proof.
 Qed.
 
 
-Fixpoint mark (fuel:nat) (r: roots_t) (h: heap_t) : set ptr :=
+Fixpoint mark (r: roots_t) (h: heap_t) : set ptr :=
   match r with
   | List.nil => List.nil
   | List.cons (var, ptr) rest =>
-    set_union ptr_eq_dec (mark fuel rest h) (mark_ptr fuel ptr h)
+    set_union ptr_eq_dec (mark rest h) (mark_ptr (length h) ptr h)
   end
 .
 
@@ -142,37 +772,33 @@ Fixpoint sweep (h: heap_t) (ptrs: set ptr) : heap_t :=
   end
 .
 
-Definition gc (f: nat) (r: roots_t) (h: heap_t) : heap_t :=
-  sweep h (mark f r h)
+Definition gc (r: roots_t) (h: heap_t) : heap_t :=
+  sweep h (mark r h)
 .
 
 Theorem heap_marks :
-  forall address s v p p',
-    roots_maps (roots s) v p ->
-    addresses (heap s) p address p' ->
-    exists f, set_In p' (mark f (roots s) (heap s))
+  forall address roots heap var ptr ptr',
+    roots_maps roots var ptr ->
+    addresses heap ptr address ptr' ->
+    set_In ptr' (mark roots heap)
 .
 Proof.
   Hint Resolve set_union_iff.
-  intros address s.
-  induction (roots s).
+  intros address r.
+  induction r.
   * crush.
   * intros.
     destruct a.
-    specialize IHr with v p p'.
+    specialize IHr with h v p p'.
     unfold roots_maps in *.
     specialize (in_inv H). intros.
     destruct H1.
     - clear H. injection H1. clear H1. intros. subst.
       unfold mark. fold mark.
-      specialize (mark_ptr_marks address (heap s) p p' H0).
+      specialize (mark_ptr_marks address h p p' H0).
       intros.
-      inversion H. clear H.
-      exists x.
       eapply set_union_intro2. auto.
     - intuition.
-      inversion H3. clear H3.
-      exists x.
       crush.
       + apply set_union_iff.
         crush.
@@ -180,17 +806,170 @@ Proof.
         crush.
 Qed.
 
+
+Lemma pointer_equivalence :
+  forall address r h v p p' h',
+    roots_maps r v p ->
+    addresses h p address p' ->
+    sweep h (mark r h) = h' ->
+    addresses h' p address p'.
+Proof.
+  induction address.
+  * intros.
+    specialize (heap_marks TermStr r h v p p' H H0).
+    intros.
+    inversion H0. subst.
+    constructor.
+    destruct H3.
+    exists x.
+    induction h ; crush.
+    destruct a.
+    destruct (ptr_eq_dec p p'). subst.
+    - unfold heap_maps_struct in H1. unfold heap_get_struct in H1.
+      destruct (ptr_eq_dec p' p') ; crush.
+      assert (set_mem ptr_eq_dec p' (mark r ((p', x) :: h)) = true).
+      eapply set_mem_correct2. auto.
+      crush.
+      unfold heap_maps_struct. unfold heap_get_struct.
+      destruct (ptr_eq_dec p' p') ; crush.
+    - assert (set_mem ptr_eq_dec p (mark r ((p, l) :: h)) = true).
+      unfold mark.
+      induction r. crush.
+      destruct a.
+      destruct (ptr_eq_dec p0 p).
+      + subst.
+        eapply set_mem_correct2.
+        eapply set_union_intro2.
+        assert (length ((p, l) :: h) = S (length h)). crush.
+        rewrite H3. clear H3.
+        unfold mark_ptr. fold mark_ptr.
+        unfold heap_get_struct. fold heap_get_struct.
+        destruct (ptr_eq_dec p p) ; crush.
+        eapply set_union_intro1. crush.
+      + assert (roots_maps r v p'). unfold roots_maps in *. unfold In in H.
+        destruct H. injection H. intros. rewrite H3 in n0.
+        assert (addresses h p' TermStr p').
+
+
+    eapply TermAddresses.
+
+    constructor.
+    eapply heap_marks.
+Qed.
+
 (* Must be proved for liveness *)
 Lemma pointer_equivalence :
   forall address s v p p' h,
     roots_maps (roots s) v p ->
     addresses (heap s) p address p' ->
-    sweep (heap s) (mark (fuel s) (roots s) (heap s)) = h ->
+    sweep (heap s) (mark (roots s) (heap s)) = h ->
     addresses h p address p'.
 Proof.
-(*  induction address.
+  induction address.
   * intros.
-    inversion H0.
+    inversion H0; subst.
+    destruct H2.
+    constructor.
+    exists x.
+    induction (heap s); crush.
+    destruct a.
+    unfold heap_maps_struct in *.
+    destruct (ptr_eq_dec p p') eqn:?.
+    - crush.
+      rewrite Heqs0 in H1.
+      edestruct set_mem eqn:?.
+      + crush.
+      + contradict Heqb.
+        unfold mark.
+        crush.
+        clear - H2 H.
+        induction (roots s). crush.
+        destruct a.
+        destruct (ptr_eq_dec p p') eqn:?.
+        ** crush.
+           rewrite Heqs0 in H2.
+           specialize (set_mem_complete1 ptr_eq_dec p' _ H2).
+           intros. contradiction H0.
+           eapply set_union_intro2.
+           eapply set_union_intro1.
+           crush.
+        ** unfold roots_maps in *.
+           unfold In in H.
+           destruct H. crush.
+           intuition.
+           remember ((fix mark (r : roots_t) (h : heap_t) {struct r} :
+           set ptr :=
+             match r with
+             | nil => nil
+             | (_, ptr0) :: rest =>
+                 set_union ptr_eq_dec (mark rest h) (mark_ptr (length h) ptr0 h)
+             end) r ((p', x) :: h)) as foo.
+           clear - H0 H2.
+           assert (set_mem ptr_eq_dec p' foo = true).
+           destruct (set_In_dec ptr_eq_dec p' foo). eapply set_mem_correct2. auto.
+           specialize (set_mem_complete2 ptr_eq_dec p' foo n). auto.
+           specialize (set_mem_correct1 ptr_eq_dec p' foo H). intros.
+           specialize (set_mem_complete1 ptr_eq_dec p' _ H2). intros.
+           contradict H3.
+           eapply set_union_intro1. auto.
+    - assert (addresses h p' TermStr p').
+      constructor. unfold heap_maps_struct.
+      exists x.
+      crush.
+      rewrite Heqs0 in H1. crush.
+      intuition.
+      assert (heap_get_struct p' h = Some x). crush. rewrite Heqs0 in H1. crush.
+      intuition.
+      edestruct set_mem eqn:?.
+      + unfold heap_get_struct. rewrite Heqs0. fold heap_get_struct.
+        admit.
+      + admit.
+
+      edestruct set_mem eqn:?.
+
+           specialize (set_mem_complete1 ptr_eq_dec p' _ H0).
+           unfold not.
+           intros.
+           assert (set_mem ptr_eq_dec p' foo = true).
+           unfo
+           crush.
+           contradict H1.
+           eapply set_union_intro1.
+           contradict H0.
+           crush.
+           unfold not in H1.
+           eapply H0 in H1.
+
+        unfold not. intros.
+        specialize (set_mem_complete1 ptr_eq_dec p' (set_union ptr_eq_dec
+            ((fix mark (r : roots_t) (h : heap_t) {struct r} :
+              set ptr :=
+                match r with
+                | nil => nil
+                | (_, ptr0) :: rest =>
+                    set_union ptr_eq_dec (mark rest h) (mark_ptr (length h) ptr0 h)
+                end) r ((p', l) :: h))
+            (mark_ptr (length ((p', l) :: h)) p ((p', l) :: h))) H2).
+        intros.
+        contradiction H3.
+
+        unfold mark_ptr.
+        assert ((length ((p', l) :: h)) = S (length h)). crush.
+        rewrite H4.
+        unfold hea
+
+
+      edestruct set_mem.
+    - unfold heap_maps_struct in *.
+      crush.
+      edestruct ptr_eq_dec. crush.
+      intuition.
+    unfold sweep.
+
+    eexists. apply H1.
+    crush.
+    inversion H2.
+    inversion H5.
   * intros.
     inversion H0.
     subst.
